bunch of plumbing

src/StepLib.v
@@ -1,42 +1,98 @@
 
 
-Inductive sstar {state : Type} (sstep : state -> state -> Prop) : state -> state -> Prop :=
-| SStarNil : forall e, sstar sstep e e
+Section steplib.
+
+Variable state : Type.
+Variable sstep : state -> state -> Prop.
+
+
+Inductive sstar : state -> state -> Prop :=
+| SStarNil : forall e, sstar e e
 | SStarCons : forall e e' e'',
         sstep e e' ->
-        sstar sstep e' e'' ->
-        sstar sstep e e''.
+        sstar e' e'' ->
+        sstar e e''.
 
-Inductive splus {state : Type} (sstep : state -> state -> Prop) : state -> state -> Prop :=
+Inductive splus  : state -> state -> Prop :=
 | SPlusOne : forall s s',
         sstep s s' ->
-        splus sstep s s'
+        splus s s'
 | SPlusCons : forall s s' s'',
         sstep s s' ->
-        splus sstep s' s'' ->
-        splus sstep s s''.
+        splus s' s'' ->
+        splus s s''.
 
 
+Lemma sstar_snoc : forall s s' s'',
+    sstar s s' ->
+    sstep s' s'' ->
+    sstar s s''.
+induction 1; intros.
+- econstructor; try eassumption. econstructor.
+- econstructor; eauto.
+Qed.
+
+Lemma splus_snoc : forall s s' s'',
+    splus s s' ->
+    sstep s' s'' ->
+    splus s s''.
+induction 1; intros.
+- econstructor 2; try eassumption.
+  econstructor 1; eassumption.
+- econstructor; solve [eauto].
+Qed.
+
+Lemma splus_sstar : forall s s',
+    splus s s' ->
+    sstar s s'.
+induction 1; intros.
+- econstructor; try eassumption. constructor.
+- econstructor; eauto.
+Qed.
+
+Lemma sstar_then_sstar : forall s s' s'',
+    sstar s s' ->
+    sstar s' s'' ->
+    sstar s s''.
+induction 1; intros.
+- assumption.
+- econstructor; solve [eauto].
+Qed.
+
+Lemma sstar_then_splus : forall s s' s'',
+    sstar s s' ->
+    splus s' s'' ->
+    splus s s''.
+induction 1; intros.
+- assumption.
+- econstructor; solve [eauto].
+Qed.
+
+Lemma splus_then_sstar' : forall s s' s'',
+    sstar s' s'' ->
+    splus s s' ->
+    splus s s''.
+induction 1; intros.
+- assumption.
+- eapply IHsstar. eapply splus_snoc; eauto.
+Qed.
+
+Lemma splus_then_sstar : forall s s' s'',
+    splus s s' ->
+    sstar s' s'' ->
+    splus s s''.
+intros. eauto using splus_then_sstar'.
+Qed.
+
+Lemma splus_then_splus : forall s s' s'',
+    splus s s' ->
+    splus s' s'' ->
+    splus s s''.
+induction 1; intros; eauto using SPlusCons.
+Qed.
+
+End steplib.
 
 
-(* Inductive sstar {A : Type} (step : A -> A -> Prop) : A -> A -> Prop := *)
-(* | star_refl : *)
-(*     forall st, *)
-(*       simple_star step st st *)
-(* | star_left : *)
-(*     forall st1 st2 st3, *)
-(*       step st1 st2 -> *)
-(*       simple_star step st2 st3 -> *)
-(*       simple_star step st1 st3. *)
-
-(* Inductive splus {A : Type} (step : A -> A -> Prop) : A -> A -> Prop := *)
-(* | plus_one : *)
-(*     forall st st', *)
-(*       step st st' -> *)
-(*       simple_plus step st st' *)
-(* | plus_left : *)
-(*     forall st1 st2 st3, *)
-(*       step st1 st2 -> *)
-(*       simple_plus step st2 st3 -> *)
-(*       simple_plus step st1 st3. *)
-
+Implicit Arguments sstar [state].
+Implicit Arguments splus [state].
